$$
f(x)^4 A(a|f(a))
$$
$$

$$

$$
$$
f(a)=a^4 -> A(a|a^4)

Schritt 1:
F(x)^3
F(a+h) = (a+h)^4
$$ B(a+h | a^4+4*a^3*h+6*a^2*h^+4*a*h^3+h^4)
$$
$$  a^4+4*a^3*h+6*a^2*h^+4*a*h^3+h^4-a^4 / a+h -a
$$
$$ 4*a^3*h+6*a^2*h^+4*a*h^3+h^4-a^4 / h
$$
$$ h(4*a^3+6*a^2*h^3*a*h^2+h^3-a^4) /h
$$
$$ 4*a^3+6*a^2*h^3*a*h^2+h^3
$$
lim H -> 0
$$ 4*a^3+6*a^2*0^3*a*0^2+0^3
$$
$$ M= 4*a^3
$$F(x)x^2+3x
F(x)2^2+6
F(x)=10


Schritt 1:
X = 2 + h
f(2+h) = x^2+3x
f(2+h) = (2+h)^2+3x
f(2+h) = (2+h)^2+3*(2+h)
f(2+h) = h^2 +7 * h+10